More documentation.

theories/DVE.v
@@ -4,7 +4,9 @@ Require Import IL Annotation LabelsDefined Sawtooth InRel Liveness TrueLiveness.
 Set Implicit Arguments.
 Unset Printing Records.
 
-Definition filter (Z:params) (lv:set var) := List.filter (fun x => B[x ∈ lv]) Z.
+(** ** Dead Variable Elimination *)
+
+Definition filter_set (Z:params) (lv:set var) := List.filter (fun x => B[x ∈ lv]) Z.
 
 Fixpoint compile (LV:list ((set var) * params)) (s:stmt) (a:ann (set var)) :=
   match s, a with
@@ -25,197 +27,13 @@ Fixpoint compile (LV:list ((set var) * params)) (s:stmt) (a:ann (set var)) :=
     | stmtReturn x, ann0 _ => stmtReturn x
     | stmtFun F t, annF lv ans ant =>
       let LV' := pair ⊜ (getAnn ⊝ ans) (fst ⊝ F) ++ LV in
-      stmtFun (zip (fun Zs a => (filter (fst Zs) (getAnn a), compile LV' (snd Zs) a)) F ans)
+      stmtFun (zip (fun Zs a => (filter_set (fst Zs) (getAnn a), compile LV' (snd Zs) a)) F ans)
               (compile LV' t ant)
     | s, _ => s
   end.
 
-Lemma getAnn_eq X Y Y' (F:list (Y * Y')) (als:list (ann X))
-  : ❬F❭ = ❬als❭
-    -> getAnn ⊝ als = fst ⊝ pair ⊜ (getAnn ⊝ als) (fst ⊝ F).
-Proof.
-  intros LEN.
-  rewrite map_zip.
-  rewrite zip_map_fst; eauto with len.
-Qed.
 
-Lemma getAnn_take_eq X Y Y' (F:list (Y * Y')) (als:list (ann X)) k a LV
-  : ❬F❭ = ❬als❭
-    -> get als k a
-    -> getAnn ⊝ take k als = fst ⊝ take k (pair ⊜ (getAnn ⊝ als) (fst ⊝ F) ++ LV).
-Proof.
-  intros LEN Get.
-  rewrite take_app_lt; eauto with len.
-  repeat rewrite map_take.
-  rewrite map_zip.
-  rewrite zip_map_fst; eauto with len.
-Qed.
-
-
-Fixpoint compile_live (s:stmt) (a:ann (set var)) (G:set var) : ann (set var) :=
-  match s, a with
-    | stmtLet x e s, ann1 lv an as a =>
-      if [x ∈ getAnn an \/ isCall e] then ann1 (G ∪ lv) (compile_live s an {x})
-                         else compile_live s an G
-    | stmtIf e s t, ann2 lv ans ant =>
-      if [op2bool e = Some true] then
-        compile_live s ans G
-      else if [op2bool e = Some false ] then
-        compile_live t ant G
-      else
-        ann2 (G ∪ lv) (compile_live s ans ∅) (compile_live t ant ∅)
-    | stmtApp f Y, ann0 lv => ann0 (G ∪ lv)
-    | stmtReturn x, ann0 lv => ann0 (G ∪ lv)
-    | stmtFun F t, annF lv ans ant =>
-      let ans' := zip (fun Zs a => let a' := compile_live (snd Zs) a ∅ in
-                               setTopAnn a' (getAnn a' ∪ of_list (filter (fst Zs) (getAnn a)))) F ans
-      in annF (G ∪ lv) ans' (compile_live t ant ∅)
-    | _, a => a
-  end.
-
-
-Lemma compile_live_incl G i ZL LV s lv
-  : true_live_sound i ZL LV s lv
-    -> getAnn (compile_live s lv G) ⊆ G ∪ getAnn lv.
-Proof.
-  intros. general induction H; simpl; eauto.
-  - cases; simpl; try reflexivity.
-    rewrite IHtrue_live_sound. rewrite <- H1. cset_tac; intuition.
-  - repeat cases; simpl; try reflexivity.
-    + etransitivity; eauto. rewrite H4; eauto.
-    + etransitivity; eauto. rewrite <- H5; eauto.
-Qed.
-
-Lemma compile_live_incl_empty i ZL LV s lv
-  : true_live_sound i ZL LV s lv
-    -> getAnn (compile_live s lv ∅) ⊆ getAnn lv.
-Proof.
-  intros.
-  eapply compile_live_incl in H.
-  rewrite H. cset_tac; intuition.
-Qed.
-
-Lemma incl_compile_live G i ZL LV s lv
-  : true_live_sound i ZL LV s lv
-    -> G ⊆ getAnn (compile_live s lv G).
-Proof.
-  intros. general induction H; simpl; eauto.
-  - cases; simpl; eauto with cset.
-  - repeat cases; simpl; eauto.
-Qed.
-
-Lemma dve_live i ZL LV s lv G
-  : true_live_sound i ZL LV s lv
-    -> live_sound i (filter ⊜ ZL LV) LV (compile (zip pair LV ZL) s lv) (compile_live s lv G).
-Proof.
-  intros. general induction H; simpl; eauto using live_sound, compile_live_incl.
-  - cases; eauto. econstructor; eauto.
-    + eapply live_exp_sound_incl; eauto.
-    + rewrite compile_live_incl; eauto.
-      rewrite <- H1. cset_tac; intuition.
-    + eapply incl_compile_live; eauto.
-  - repeat cases; eauto.
-    + econstructor; eauto.
-      eapply live_op_sound_incl; eauto.
-      rewrite compile_live_incl_empty; eauto with cset.
-      rewrite compile_live_incl_empty; eauto with cset.
-  - econstructor; eauto using zip_get.
-    + simpl. cases; eauto.
-      rewrite <- H1. rewrite minus_inter_empty. eapply incl_right.
-      unfold filter. rewrite of_list_filter.
-      cset_tac; intuition.
-    + erewrite get_nth; eauto using zip_get.
-      simpl. eauto with len.
-    + intros ? ? Get. erewrite get_nth in Get; eauto using zip_get. simpl in *.
-      edestruct filter_by_get as [? [? []]]; eauto; dcr. simpl in *; cases in H6.
-      eapply live_op_sound_incl.
-      eapply argsLive_live_exp_sound; eauto. eauto with cset.
-  - econstructor; eauto.
-    eapply live_op_sound_incl; eauto using incl_right.
-  - econstructor; simpl in *; eauto with len.
-    + eapply live_sound_monotone.
-      rewrite map_zip. simpl.
-      do 2 rewrite zip_app in IHtrue_live_sound; eauto with len.
-      rewrite zip_map_l, zip_map_r in IHtrue_live_sound.
-      eapply IHtrue_live_sound.
-      eapply PIR2_app; eauto.
-      eapply PIR2_get; eauto 30 with len.
-      intros; inv_get. simpl. rewrite getAnn_setTopAnn.
-      rewrite compile_live_incl_empty; eauto. unfold filter.
-      rewrite of_list_filter. cset_tac.
-    + intros; inv_get. simpl.
-      eapply live_sound_monotone.
-      eapply live_sound_monotone2; eauto.
-      rewrite map_zip. simpl.
-      do 2 rewrite zip_app in H2; eauto with len.
-      rewrite zip_map_l, zip_map_r in H2.
-      eapply H2; eauto.
-      eapply PIR2_app; eauto.
-      eapply PIR2_get; eauto 30 with len.
-      intros; inv_get. simpl. rewrite getAnn_setTopAnn.
-      rewrite compile_live_incl_empty; eauto.
-      unfold filter. rewrite of_list_filter. cset_tac.
-    + intros; inv_get.
-      repeat rewrite getAnn_setTopAnn; simpl.
-      split; eauto. cases; eauto.
-      exploit H3; eauto.
-      rewrite compile_live_incl_empty; eauto. rewrite <- H5.
-      unfold filter. rewrite of_list_filter. clear_all; cset_tac.
-    + rewrite compile_live_incl; eauto with cset.
-Qed.
-
-Lemma DVE_callChain Lv ZL F als n l'
-  : ❬F❭ = ❬als❭
-    -> (forall (n : nat) (Zs : params * stmt) (a : ann ⦃var⦄),
-         get F n Zs ->
-         get als n a ->
-         forall n0 : nat,
-           trueIsCalled (snd Zs) (LabI n0) ->
-           trueIsCalled (compile (pair ⊜ (getAnn ⊝ als ++ Lv) (fst ⊝ F ++ ZL)) (snd Zs) a) (LabI n0))
-     -> callChain trueIsCalled F (LabI l') (LabI n)
-     -> callChain trueIsCalled
-                 ((fun (Zs : params * stmt) (a : ann ⦃var⦄) =>
-                     (filter (fst Zs) (getAnn a),
-                      compile (pair ⊜ (getAnn ⊝ als ++ Lv) (fst ⊝ F ++ ZL)) (snd Zs) a)) ⊜ F als)
-                 (LabI l') (LabI n).
-Proof.
-  intros LEN IH CC.
-  general induction CC.
-  + econstructor.
-  + inv_get. econstructor 2.
-    eapply zip_get; eauto.
-    eapply IH; eauto.
-    eauto.
-Qed.
-
-Lemma DVE_isCalled i ZL LV s lv n
-  : true_live_sound i ZL LV s lv
-    -> trueIsCalled s (LabI n)
-    -> trueIsCalled (compile (zip pair LV ZL) s lv) (LabI n).
-Proof.
-  intros LS IC.
-  general induction LS; invt trueIsCalled; simpl; repeat cases; eauto using trueIsCalled;
-    try congruence.
-  - destruct l' as [l'].
-    econstructor; rewrite <- zip_app; eauto with len.
-    rewrite zip_length2; eauto. eapply DVE_callChain; eauto.
-Qed.
-
-Lemma DVE_noUnreachableCode i ZL LV s lv
-  : true_live_sound i ZL LV s lv
-    -> noUnreachableCode trueIsCalled s
-    -> noUnreachableCode trueIsCalled (compile (zip pair LV ZL) s lv).
-Proof.
-  intros LS UC.
-  general induction LS; inv UC; simpl; repeat cases; eauto using noUnreachableCode.
-  - econstructor; intros; inv_get; rewrite <- zip_app; simpl; eauto with len.
-    + edestruct H8 as [[l] [IC CC]]. rewrite zip_length2 in H4; eauto.
-      eexists (LabI l); split; eauto.
-      eapply DVE_isCalled; eauto.
-      eapply DVE_callChain; eauto using DVE_isCalled.
-Qed.
-
-Require Import BisimSim.
+(** ** Correctness with respect to the imperative semantics IL/I *)
 
 Module I.
 
@@ -223,7 +41,7 @@ Module I.
 
 
 Instance SR : PointwiseProofRelationI ((set var) * params) := {
-   ParamRelIP G Z Z' := Z' = (List.filter (fun x => B[x ∈ fst G]) Z) /\ snd G = Z;
+   ParamRelIP G Z Z' := Z' = (filter (fun x => B[x ∈ fst G]) Z) /\ snd G = Z;
    ArgRelIP V V' G VL VL' :=
      VL' = (filter_by (fun x => B[x ∈ fst G]) (snd G) VL) /\
      length (snd G) = length VL /\
@@ -290,12 +108,15 @@ Qed.
 
 End I.
 
+(** ** Correctness with respect to the functional semantics IL *)
+(** Functional here means that variables are lexically scoped binders instead of assignables. *)
+
 Module F.
 
   Require Import SimF.
 
 Instance SR : PointwiseProofRelationF ((set var) * params) := {
-   ParamRelFP G Z Z' := Z' = (List.filter (fun x => B[x ∈ fst G]) Z) /\ snd G = Z;
+   ParamRelFP G Z Z' := Z' = (filter (fun x => B[x ∈ fst G]) Z) /\ snd G = Z;
    ArgRelFP G VL VL' :=
      VL' = (filter_by (fun x => B[x ∈ fst G]) (snd G) VL) /\
      length (snd G) = length VL
@@ -359,3 +180,176 @@ Proof.
 Qed.
 
 End F.
+
+
+(** ** Reconstruction of Liveness Information after DVE *)
+(** In this section we show that liveness information can
+    be transformed alongside DVE.
+    This means that liveness recomputation after the transformation is not neccessary. *)
+
+
+Fixpoint compile_live (s:stmt) (a:ann (set var)) (G:set var) : ann (set var) :=
+  match s, a with
+    | stmtLet x e s, ann1 lv an as a =>
+      if [x ∈ getAnn an \/ isCall e] then ann1 (G ∪ lv) (compile_live s an {x})
+                         else compile_live s an G
+    | stmtIf e s t, ann2 lv ans ant =>
+      if [op2bool e = Some true] then
+        compile_live s ans G
+      else if [op2bool e = Some false ] then
+        compile_live t ant G
+      else
+        ann2 (G ∪ lv) (compile_live s ans ∅) (compile_live t ant ∅)
+    | stmtApp f Y, ann0 lv => ann0 (G ∪ lv)
+    | stmtReturn x, ann0 lv => ann0 (G ∪ lv)
+    | stmtFun F t, annF lv ans ant =>
+      let ans' := zip (fun Zs a => let a' := compile_live (snd Zs) a ∅ in
+                               setTopAnn a' (getAnn a' ∪ of_list (filter_set (fst Zs) (getAnn a)))) F ans
+      in annF (G ∪ lv) ans' (compile_live t ant ∅)
+    | _, a => a
+  end.
+
+
+Lemma compile_live_incl G i ZL LV s lv
+  : true_live_sound i ZL LV s lv
+    -> getAnn (compile_live s lv G) ⊆ G ∪ getAnn lv.
+Proof.
+  intros. general induction H; simpl; eauto.
+  - cases; simpl; try reflexivity.
+    rewrite IHtrue_live_sound. rewrite <- H1. cset_tac; intuition.
+  - repeat cases; simpl; try reflexivity.
+    + etransitivity; eauto. rewrite H4; eauto.
+    + etransitivity; eauto. rewrite <- H5; eauto.
+Qed.
+
+Lemma compile_live_incl_empty i ZL LV s lv
+  : true_live_sound i ZL LV s lv
+    -> getAnn (compile_live s lv ∅) ⊆ getAnn lv.
+Proof.
+  intros.
+  eapply compile_live_incl in H.
+  rewrite H. cset_tac; intuition.
+Qed.
+
+Lemma incl_compile_live G i ZL LV s lv
+  : true_live_sound i ZL LV s lv
+    -> G ⊆ getAnn (compile_live s lv G).
+Proof.
+  intros. general induction H; simpl; eauto.
+  - cases; simpl; eauto with cset.
+  - repeat cases; simpl; eauto.
+Qed.
+
+Lemma dve_live i ZL LV s lv G
+  : true_live_sound i ZL LV s lv
+    -> live_sound i (filter_set ⊜ ZL LV) LV (compile (zip pair LV ZL) s lv) (compile_live s lv G).
+Proof.
+  intros. general induction H; simpl; eauto using live_sound, compile_live_incl.
+  - cases; eauto. econstructor; eauto.
+    + eapply live_exp_sound_incl; eauto.
+    + rewrite compile_live_incl; eauto.
+      rewrite <- H1. cset_tac; intuition.
+    + eapply incl_compile_live; eauto.
+  - repeat cases; eauto.
+    + econstructor; eauto.
+      eapply live_op_sound_incl; eauto.
+      rewrite compile_live_incl_empty; eauto with cset.
+      rewrite compile_live_incl_empty; eauto with cset.
+  - econstructor; eauto using zip_get.
+    + simpl. cases; eauto.
+      rewrite <- H1. rewrite minus_inter_empty. eapply incl_right.
+      unfold filter_set. rewrite of_list_filter.
+      cset_tac; intuition.
+    + erewrite get_nth; eauto using zip_get.
+      simpl. eauto with len.
+    + intros ? ? Get. erewrite get_nth in Get; eauto using zip_get. simpl in *.
+      edestruct filter_by_get as [? [? []]]; eauto; dcr. simpl in *; cases in H6.
+      eapply live_op_sound_incl.
+      eapply argsLive_live_exp_sound; eauto. eauto with cset.
+  - econstructor; eauto.
+    eapply live_op_sound_incl; eauto using incl_right.
+  - econstructor; simpl in *; eauto with len.
+    + eapply live_sound_monotone.
+      rewrite map_zip. simpl.
+      do 2 rewrite zip_app in IHtrue_live_sound; eauto with len.
+      rewrite zip_map_l, zip_map_r in IHtrue_live_sound.
+      eapply IHtrue_live_sound.
+      eapply PIR2_app; eauto.
+      eapply PIR2_get; eauto 30 with len.
+      intros; inv_get. simpl. rewrite getAnn_setTopAnn.
+      rewrite compile_live_incl_empty; eauto. unfold filter_set.
+      rewrite of_list_filter. cset_tac.
+    + intros; inv_get. simpl.
+      eapply live_sound_monotone.
+      eapply live_sound_monotone2; eauto.
+      rewrite map_zip. simpl.
+      do 2 rewrite zip_app in H2; eauto with len.
+      rewrite zip_map_l, zip_map_r in H2.
+      eapply H2; eauto.
+      eapply PIR2_app; eauto.
+      eapply PIR2_get; eauto 30 with len.
+      intros; inv_get. simpl. rewrite getAnn_setTopAnn.
+      rewrite compile_live_incl_empty; eauto.
+      unfold filter_set. rewrite of_list_filter. cset_tac.
+    + intros; inv_get.
+      repeat rewrite getAnn_setTopAnn; simpl.
+      split; eauto. cases; eauto.
+      exploit H3; eauto.
+      rewrite compile_live_incl_empty; eauto. rewrite <- H5.
+      unfold filter_set. rewrite of_list_filter. clear_all; cset_tac.
+    + rewrite compile_live_incl; eauto with cset.
+Qed.
+
+(** ** DVE and Unreachable Code *)
+(** We show that DVE does not introduce unreachable code. *)
+
+Lemma DVE_callChain Lv ZL F als n l'
+  : ❬F❭ = ❬als❭
+    -> (forall (n : nat) (Zs : params * stmt) (a : ann ⦃var⦄),
+         get F n Zs ->
+         get als n a ->
+         forall n0 : nat,
+           trueIsCalled (snd Zs) (LabI n0) ->
+           trueIsCalled (compile (pair ⊜ (getAnn ⊝ als ++ Lv) (fst ⊝ F ++ ZL)) (snd Zs) a) (LabI n0))
+     -> callChain trueIsCalled F (LabI l') (LabI n)
+     -> callChain trueIsCalled
+                 ((fun (Zs : params * stmt) (a : ann ⦃var⦄) =>
+                     (filter_set (fst Zs) (getAnn a),
+                      compile (pair ⊜ (getAnn ⊝ als ++ Lv) (fst ⊝ F ++ ZL)) (snd Zs) a)) ⊜ F als)
+                 (LabI l') (LabI n).
+Proof.
+  intros LEN IH CC.
+  general induction CC.
+  + econstructor.
+  + inv_get. econstructor 2.
+    eapply zip_get; eauto.
+    eapply IH; eauto.
+    eauto.
+Qed.
+
+Lemma DVE_isCalled i ZL LV s lv n
+  : true_live_sound i ZL LV s lv
+    -> trueIsCalled s (LabI n)
+    -> trueIsCalled (compile (zip pair LV ZL) s lv) (LabI n).
+Proof.
+  intros LS IC.
+  general induction LS; invt trueIsCalled; simpl; repeat cases; eauto using trueIsCalled;
+    try congruence.
+  - destruct l' as [l'].
+    econstructor; rewrite <- zip_app; eauto with len.
+    rewrite zip_length2; eauto. eapply DVE_callChain; eauto.
+Qed.
+
+Lemma DVE_noUnreachableCode i ZL LV s lv
+  : true_live_sound i ZL LV s lv
+    -> noUnreachableCode trueIsCalled s
+    -> noUnreachableCode trueIsCalled (compile (zip pair LV ZL) s lv).
+Proof.
+  intros LS UC.
+  general induction LS; inv UC; simpl; repeat cases; eauto using noUnreachableCode.
+  - econstructor; intros; inv_get; rewrite <- zip_app; simpl; eauto with len.
+    + edestruct H8 as [[l] [IC CC]]. rewrite zip_length2 in H4; eauto.
+      eexists (LabI l); split; eauto.
+      eapply DVE_isCalled; eauto.
+      eapply DVE_callChain; eauto using DVE_isCalled.
+Qed.
